src/util/meta/tactic/propositional.lean
@@ -21,21 +21,6 @@ meta def try_abstract (e : expr) : tactic (list expr) :=
 open nat smt_tactic (eblast solve_goals)
 open smt_tactic.interactive (rsimp)
 
-meta def split_or (xs : list expr) : smt_tactic (list expr) :=
-do cs ← local_context,
-   h ← mmap (λ h, try_core $ do
-     t ← infer_type h,
-     h <$ (match_or t <|> match_and t))
-   $ cs.diff xs,
-  let h' := h.filter_map id,
-  h' <$ mmap' smt_tactic.destruct h'
-
-meta def split_all_or' : list expr → smt_tactic unit
- | xs := do ys ← split_or xs, (guard (¬ ys.empty) >> smt_tactic.all_goals (split_all_or' (ys ++ xs))) <|> return ()
-
-meta def split_all_or : smt_tactic unit :=
-split_all_or' []
-
 meta def show_prop : tactic unit :=
 -- do p ← target,
 --    vs ← list.join <$> mmap try_abstract (atoms p).to_list,
@@ -56,8 +41,5 @@ do t ← target,
   end
 
 end tactic
-
-meta def smt_tactic.interactive.break_asms : smt_tactic unit :=
-tactic.split_all_or
 
 run_cmd add_interactive [`tactic.propositional]
